start proof

simpleversionTree.dfy
@@ -5,21 +5,17 @@ datatype FoodTree =
 datatype LabeledTree = 
   LabeledNode(name: string, labelname: string, children: seq<LabeledTree>)
 
-function IsIngredientSafe(name: string, allergens: set<string>): bool
-{
-  name !in allergens
-}
-
-function AllIngredients(t: FoodTree): set<string>
-{
+predicate AllergenFree(t: FoodTree, allergens: set<string>) {
   match t
-  case Ingredient(name) => {name}
+  case Ingredient(name) => !(name in allergens)
   case Choice(_, children) =>
-    set ing | c := children[..], i :: 0 <= i < |children|, ing in AllIngredients(children[i]) :: true
+    forall child :: child in children ==> AllergenFree(child, allergens)
 }
 
 method LabelTree(t: FoodTree, allergens: set<string>) returns (lt: LabeledTree)
-  ensures lt.labelname == "safe" <==> (t.AllIngredients(t) * allergens) == {}
+  ensures lt.labelname in {"safe", "not safe"}
+  ensures lt.name == t.name
+  ensures lt.labelname == "safe" <==> AllergenFree(t, allergens)
 {
   match t
   //label for leaf node (node doesn't have children)
@@ -28,26 +24,47 @@ method LabelTree(t: FoodTree, allergens: set<string>) returns (lt: LabeledTree)
       lt := LabeledNode(name, "not safe", []);
     } else {
       lt := LabeledNode(name, "safe", []);
+      assert t == Ingredient(name);
+      assert !(name in allergens);
+      assert AllergenFree(t, allergens);
     }
 
   //label for nodes that have children
   case Choice(name, children) =>
     var labeledChildren: seq<LabeledTree> := [];
+    ghost var processedChildren: seq<FoodTree> := [];
     var anyUnsafe := false;
 
     var i := 0;
     while i < |children|
       invariant 0 <= i <= |children|
       invariant |labeledChildren| == i
+      invariant forall labeledChild :: labeledChild in labeledChildren
+                  ==> labeledChild.labelname in {"safe", "not safe"}
+      invariant |labeledChildren| == |processedChildren|
+      invariant forall i: nat :: 0 < i < |processedChildren|
+                  ==> labeledChildren[i].name == processedChildren[i].name
+      invariant forall i :: 0 <= i < |processedChildren|
+                  ==> (labeledChildren[i].labelname == "not safe" <==> !AllergenFree(processedChildren[i], allergens))
+      invariant forall i :: 0 <= i < |processedChildren|
+                  ==> (processedChildren[i] == children[i])
       decreases |children| - i
     {
-      var childLabeled := LabelTree(children[i], allergens);
+      var child := children[i];
+      var childLabeled := LabelTree(child, allergens);
       if childLabeled.labelname == "not safe" {
         anyUnsafe := true;
       }
       labeledChildren := labeledChildren + [childLabeled];
+      processedChildren := processedChildren + [child];
       i := i + 1;
     }
+    assert |processedChildren| == |children|;
+    assert forall i :: 0 <= i < |children|
+                  ==> (processedChildren[i] == children[i]);
+    assert processedChildren == children;
+    assert forall i :: 0 <= i < |children|
+            ==> (labeledChildren[i].labelname == "not safe" <==> !AllergenFree(processedChildren[i], allergens));
 
     var labelN := if anyUnsafe then "not safe" else "safe";
     lt := LabeledNode(name, labelN, labeledChildren);
